theories/case_studies/asynchronous.v
@@ -13,7 +13,7 @@ From hazel.program_logic Require Import weakest_precondition
 
 (* Local imports *)
 From haffel.lib Require Import base.
-From haffel.lang Require Import hazel.
+From haffel.lang Require Import haffel.
 From haffel.logic Require Import sem_def.
 From haffel.logic Require Import sem_env.
 From haffel.logic Require Import sem_types.
