theories/logic/mode.v
@@ -1,0 +1,62 @@
+
+From iris.proofmode Require Import base tactics.
+From iris.algebra Require Import ofe gmap.
+From iris.base_logic Require Export iprop upred invariants.
+
+(* Hazel Reasoning *)
+From hazel.program_logic Require Import weakest_precondition 
+                                        state_reasoning
+                                        protocols.
+
+(* Local imports *)
+From haffel.lib Require Import logic.
+From haffel.lang Require Import haffel.
+From haffel.lang Require Import subst_map.
+From haffel.logic Require Import iEff.
+From haffel.logic Require Import sem_def.
+
+Definition mode_mult m m' : mode :=
+  match m with
+    MS => MS
+  | OS => m'
+  end.
+
+Lemma mode_mult_idemp m :
+  mode_mult m m = m.
+Proof. by destruct m. Qed.
+
+Lemma mode_mult_assoc m₁ m₂ m₃ :
+  mode_mult m₁ (mode_mult m₂ m₃) = (mode_mult (mode_mult m₁ m₂) m₃).
+Proof. by destruct m₁. Qed.
+
+Lemma mode_mult_comm m₁ m₂ :
+  mode_mult m₁ m₂ = mode_mult m₂ m₁.
+Proof. by destruct m₁, m₂. Qed.
+
+Lemma mode_mult_ms m :
+  mode_mult MS m = MS.
+Proof. destruct m; eauto. Qed.
+
+(* Sub-Typing on Mode *)
+
+Lemma mode_le_refl {Σ} (m : mode) : ⊢ (m ≤M m : iProp Σ).
+Proof. by iLeft. Qed.
+
+Lemma mode_le_trans {Σ} (m1 m2 m3 : mode) : 
+  m1 ≤M m2 -∗
+  m2 ≤M m3 -∗
+  (m1 ≤M m3 : iProp Σ).
+Proof. iIntros "#H12 H23". destruct m1,m2,m3; eauto. Qed.
+
+Lemma mode_le_MS {Σ} (m : mode) : 
+  ⊢ (MS ≤M m : iProp Σ).
+Proof. by iRight. Qed.
+
+Lemma mode_mult_le {Σ} (m₁ m₁' m₂ m₂' : mode) :
+  m₁ ≤M m₁' -∗ m₂ ≤M m₂' -∗
+  mode_mult m₁ m₂ ≤M@{ Σ } mode_mult m₁' m₂'.
+Proof. iIntros "Hm₁₁' Hm₂₂'". destruct m₁,m₂,m₁',m₂'; eauto. Qed.
+
+Lemma mode_le_OS {Σ} (m : mode) : 
+  ⊢ (m ≤M OS : iProp Σ).
+Proof. destruct m; eauto. Qed.
