theories/logic/sem_env.v
@@ -10,7 +10,7 @@ From hazel.program_logic Require Import weakest_precondition
 
 (* Local imports *)
 From haffel.lib Require Import base.
-From haffel.lang Require Import hazel.
+From haffel.lang Require Import haffel.
 From haffel.lang Require Import subst_map.
 From haffel.logic Require Import iEff.
 From haffel.logic Require Import sem_def.
