theories/logic/sem_row.v
@@ -1,0 +1,524 @@
+
+(* sem_row.v *)
+
+(* This file contains the definition of semantic rows. *)
+
+From iris.proofmode Require Import base tactics.
+From iris.algebra Require Import ofe gmap.
+From iris.base_logic Require Export iprop upred invariants.
+
+(* Hazel Reasoning *)
+From hazel.program_logic Require Import weakest_precondition 
+                                        state_reasoning
+                                        protocols.
+
+(* Local imports *)
+From haffel.lib Require Import logic.
+From haffel.lang Require Import haffel.
+From haffel.lang Require Import subst_map.
+From haffel.logic Require Import iEff.
+From haffel.logic Require Import sem_def.
+From haffel.logic Require Import mode.
+From haffel.logic Require Import sem_sig.
+
+Definition sem_row_nil {Σ} : sem_row Σ := ∅. 
+Global Instance sem_row_bottom {Σ} : Bottom (sem_row Σ) := sem_row_nil.
+
+Definition sem_row_ins {Σ} (l : string) (σ : sem_sig Σ) (ρ : sem_row Σ) : sem_row Σ := 
+  insert (l, 0) σ ρ.
+
+Definition sem_row_os {Σ} (ρ : sem_row Σ) : sem_row Σ := 
+  fmap (λ σ, (σ.1, upcl OS σ.2)) ρ. 
+
+Definition sem_row_tun_f := (λ k : stringO * nat, (k.1, S k.2)).
+Definition sem_row_tun {Σ} (ρ : sem_row Σ) : sem_row Σ := 
+  kmap sem_row_tun_f ρ. 
+
+Local Instance inj_sem_row_tun : Inj eq eq sem_row_tun_f.
+Proof. 
+  intros k1 k2 H. 
+  rewrite /sem_row_tun_f in H. inv H.
+  destruct k1, k2. by f_equal.
+Qed.
+
+Definition sem_row_mode {Σ} (ρ : sem_row Σ) : mode := 
+  (map_fold (λ _ m acc, mode_mult acc m) OS (fst <$> ρ)).
+
+Program Definition sem_row_to_prot {Σ} (ρ : sem_row Σ) : iEff Σ :=
+  IEff (λ v, λne Φ, ∃ v' l (s : nat) σ, (v ≡ ((#(LitStr l), #s), v')%V) ∗ 
+                                lookup (l, s) ρ ≡ Some σ ∗ 
+                                iEff_car σ.2 v' Φ)%I.
+Next Obligation.
+  intros ???????. by repeat f_equiv. 
+Qed.
+
+Definition filter_row_to_os {Σ} (ρ : gmap (string * nat) (sem_sig Σ)) : sem_row Σ :=
+  union_with (λ (σ : sem_sig Σ) _, match σ.1 with 
+                        OS => Some σ
+                     |  MS => None end) ρ ρ.
+
+Instance filter_row_to_os_ne {Σ} :
+  NonExpansive (@filter_row_to_os Σ).
+Proof.
+  intros ????. rewrite /filter_row_to_os.
+  apply union_with_ne; try done.
+  intros ??????. inv H0. inv H2. rewrite H4.
+  destruct y0.1 eqn:H'; rewrite H'; last done.
+  f_equiv. destruct x0, y0. f_equiv; try done.
+  simpl in *; by subst.
+Qed.
+
+Global Instance sem_row_to_prot_ne {Σ} :
+  NonExpansive (@sem_row_to_prot Σ).
+Proof.
+  intros ????. rewrite /sem_row_to_prot. f_equiv.
+  intros ??. simpl. by repeat f_equiv.
+Qed.
+
+Global Instance sem_row_to_prot_proper {Σ} :
+  Proper ((≡) ==> (≡)) (@sem_row_to_prot Σ).
+Proof. apply ne_proper. apply _. Qed.
+
+Global Instance sem_row_mode_ne {Σ} :
+  NonExpansive (@sem_row_mode Σ).
+Proof.
+  intros n ρ ρ' H. rewrite /sem_row_mode. 
+  f_equiv. 
+  apply map_eq. intros i; rewrite !lookup_fmap.
+  destruct (ρ !! i) as [mσ|] eqn:Heq, (ρ' !! i) as [m'σ'|] eqn:Heq'; rewrite Heq Heq'.
+  - assert (H': Some mσ  ≡{n}≡ Some m'σ'). 
+    { rewrite - Heq - Heq'. apply (H i). }
+    simpl. f_equal. destruct mσ as [m σ], m'σ' as [m' σ']. 
+    inv H'. inv H2. apply leibniz_equiv; simpl in *.
+    eapply discrete_iff; [|apply H0]. apply _.
+  - assert (H' : Some mσ ≡{n}≡ None). 
+    { rewrite - Heq - Heq'. apply (H i). }
+    inv H'.
+  - assert (H' : None ≡{n}≡ Some m'σ'). 
+    { rewrite - Heq - Heq'. apply (H i). }
+    inv H'.
+  - done.
+Qed.
+
+Global Instance sem_row_mode_proper {Σ} (ρ ρ' : sem_row Σ) :
+  Proper ((≡) ==> (≡)) (@sem_row_mode Σ).
+Proof. apply ne_proper. apply _. Qed.
+
+(* Notations. *)
+
+Notation "⟨⟩" := (sem_row_nil) : sem_row_scope.
+Notation "lσ · ρ" := (sem_row_ins lσ.1 lσ.2 ρ) (at level 80, right associativity) : sem_row_scope.
+Notation "¡ ρ" := (sem_row_os ρ) (at level 10) : sem_row_scope.
+Notation "⦗ ρ ⦘" := (sem_row_tun ρ) (at level 5) : sem_row_scope.
+Notation "⟦ ρ ⟧" := (sem_row_to_prot ρ) : sem_row_scope.
+Notation "'MODE' ρ" := (sem_row_mode ρ%R) (at level 50).
+
+Lemma filter_row_to_os_lookup {Σ} (ρ : sem_row Σ) (l : string) (s : nat) (σ : sem_sig Σ) :
+  (filter_row_to_os ρ !! (l, s) ≡ Some σ : iProp Σ) ∗-∗
+  (ρ !! (l, s) ≡ Some σ ∗ σ.1 ≡ OS).
+Proof. 
+  iSplit.
+  - iIntros "H".
+    rewrite /filter_row_to_os lookup_union_with. 
+    destruct (ρ !! (l, s)) eqn:H; rewrite H /=; 
+      last (iDestruct "H" as "%H'"; inv H').
+    rewrite /union_with /=. destruct o.1 eqn:H'; rewrite H'.
+    + iDestruct (option_equivI with "H") as "#H'".
+      iRewrite - "H'". iSplit; first done. by rewrite H'.
+    + iDestruct "H" as "%H''". inv H''.
+  - iIntros "[Hlookup HσOS]". rewrite /filter_row_to_os.
+    rewrite lookup_union_with /union_with. 
+    destruct (ρ !! (l, s)) eqn:H; rewrite H /=;  
+      last (iDestruct "Hlookup" as "%H'"; inv H').
+    iDestruct (option_equivI with "Hlookup") as "#H'".
+      iRewrite - "H'" in "HσOS". by iRewrite "HσOS". 
+Qed.
+
+
+(* One-Shot Rows *)
+
+Notation OSRow ρ := (MonoProt ⟦ ρ%R ⟧)%R.
+
+Global Instance sem_row_nil_os_row {Σ} :
+  OSRow (⟨⟩ : sem_row Σ).
+Proof.
+  constructor. rewrite /sem_row_to_prot /= /sem_row_nil.
+  iIntros (v Φ Φ') "_ (% & % & % & % & _ & H & _)".
+  rewrite lookup_empty. iDestruct "H" as "%". inv H. 
+Qed.
+  
+(* TODO: This needs to be generalised, 
+         if (l, 0) ∈ ρ then ρ(l, 0) does not need to be an OSSig.
+   NOTE: we can have a separate gset of keys that we don't need to check,
+         by creating a helper class OSRow_help *)
+Global Instance sem_row_ins_os_row {Σ} (ρ : sem_row Σ) l σ `{ OSSig σ, OSRow ρ } :
+  OSRow ((l, σ) · ρ).
+Proof.
+  constructor. iIntros (v Φ Φ') "HPost".
+  rewrite /sem_row_to_prot /=.
+  iIntros "(%w & %l' & %s' & %σ' & -> & #Hlookup' & Hσ')".
+  destruct (decide ((l, 0) = (l', s'))). 
+  - rewrite /sem_row_ins. inv e. 
+    iExists w, l', 0, σ'. rewrite lookup_insert. 
+    iSplitR; first done. iFrame "#". 
+    iDestruct (option_equivI with "Hlookup'") as "#Hlookup''".
+    inv OSSig0. 
+    iDestruct (monotonic_prot w Φ Φ' with "HPost") as "H".
+    iDestruct (iEff_equivI σ.2 σ'.2) as "[Heq _]".
+    iSpecialize ("Heq" with "[]"); first by iRewrite "Hlookup''".
+    iRewrite ("Heq" $! w Φ) in "H". 
+    iRewrite ("Heq" $! w Φ') in "H". 
+    by iApply "H".
+  - inv OSRow0. rewrite /sem_row_to_prot /= in monotonic_prot.
+    iDestruct (monotonic_prot (#(LitStr l'), #s', w)%V Φ Φ' with "HPost [Hσ']") as "(%w'' & %l'' & %s'' & %σ'' & %Heq & Hlookup & Hieff)".
+    { iExists w, l', s', σ'. iSplit; first done.
+      rewrite lookup_insert_ne; last done. iFrame "∗#". }
+    inv Heq. iExists w'', l'', s'', σ''. iSplitR; first done.
+    rewrite /sem_row_ins lookup_insert_ne; last done. iFrame "∗".
+Qed.
+
+Global Instance sem_row_tun_os_row {Σ} (ρ : sem_row Σ) `{ OSRow ρ } :
+  OSRow ⦗ ρ ⦘.
+Proof.
+  constructor. rewrite /sem_row_to_prot /=. 
+  iIntros (v Φ Φ') "HPost".
+  iIntros "(% & % & % & % & #Heq & #Hlookup & Hσ)".
+  destruct s.
+  - destruct (lookup_kmap_None sem_row_tun_f ρ (l, 0)) as [_ H].
+    rewrite H; first (iDestruct "Hlookup" as "%H'"; inv H').
+    intros [l' s'] H'. inv H'. 
+  - replace (l, S s) with (sem_row_tun_f (l, s)) by done. 
+    rewrite lookup_kmap. inv OSRow0.
+    rewrite /sem_row_to_prot /= in monotonic_prot.
+    iDestruct (monotonic_prot (#(LitStr l), #s, v')%V Φ Φ' with "HPost [Hσ]") as "(%w & %l' & %s' & %σ' & Heq' & Hlookup' & Hσ')".
+    { iExists v', l, s, σ. by iFrame "#∗". }
+    iExists v', l', (S s'), σ'. iDestruct "Heq'" as "%". inv H.
+    iRewrite "Heq"; iSplitR; first done. iFrame.
+    replace (l', S s') with (sem_row_tun_f (l', s')) by done. 
+    rewrite /sem_row_tun lookup_kmap //. 
+Qed.
+
+Global Instance sem_row_os_os_row {Σ} (ρ : sem_row Σ) :
+  OSRow (¡ ρ ).
+Proof.
+  constructor. rewrite /sem_row_to_prot /=.
+  iIntros (v Φ Φ') "HPost (% & % & % & % & Heq & #Hlookup & Hσ)".
+  iExists v', l, s, σ. iFrame "∗#".
+  rewrite /sem_row_os lookup_fmap.
+  destruct (ρ !! (l, s)) eqn:H; rewrite H /=. 
+  - iDestruct (option_equivI with "Hlookup") as "#Hlookup'".
+    destruct σ. simpl.
+    iDestruct (prod_equivI with "Hlookup'") as "[_ Heq]". simpl.
+    iDestruct (iEff_equivI (upcl OS o.2) o1) as "[Heq' _]".
+    iSpecialize ("Heq'" with "Heq"). iRewrite - ("Heq'" $! v' Φ').
+    pose proof (upcl_mono_prot o.2) as [].
+    iApply (monotonic_prot with "HPost").
+    by iRewrite ("Heq'" $! v' Φ).
+  - iDestruct "Hlookup" as "%H'". inv H'.
+Qed.
+
+Global Instance sem_row_filter_row_to_os {Σ} (ρ : sem_row Σ) `{ OSRow ρ } :
+  OSRow (filter_row_to_os ρ).
+Proof.
+  constructor. iIntros (v Φ Φ') "HPost Hρ".
+  rewrite /sem_row_to_prot /=.
+  iDestruct "Hρ" as "(% & % & % & % & #Heq & #Hlookup & Hσ)".
+  iDestruct (filter_row_to_os_lookup ρ l s σ) as "[H _]".
+  iDestruct ("H" with "Hlookup") as "[Hlookup' HσOS]".
+  inv OSRow0. iPoseProof (monotonic_prot v Φ Φ' with "HPost") as "H'".
+  rewrite /sem_row_to_prot /=.
+  iDestruct ("H'" with "[Hσ]") as "(%w & %l' & %s' & %σ' & #Heq' & #Hlookup'' & Hσ')".
+  { iExists v', l, s, σ. iFrame "∗#". }
+  iExists w, l', s', σ'. iFrame "#∗".
+  iDestruct "Heq'" as "%".
+  iDestruct "Heq" as "%". inv H0. 
+  iRewrite "Hlookup''" in "Hlookup'".
+  iDestruct (option_equivI with "Hlookup'") as "#Heqσ".
+  iRewrite "Heqσ". iFrame "#".
+Qed.
+
+Lemma row_mode_nil {Σ} :
+  MODE (⟨⟩ : sem_row Σ) = OS.
+Proof. rewrite /sem_row_mode fmap_empty map_fold_empty //. Qed.
+
+Lemma row_mode_ins_delete {Σ} (x : string * nat) (σ : sem_sig Σ) (ρ : sem_row Σ) :
+  MODE (insert x σ (delete x ρ)) = mode_mult σ.1 (MODE (delete x ρ)).
+Proof.
+  rewrite /sem_row_mode fmap_insert map_fold_insert_L.
+  - by rewrite mode_mult_comm.
+  - intros ????????. rewrite - mode_mult_assoc (mode_mult_comm z2 z1) - mode_mult_assoc //.
+  - rewrite fmap_delete lookup_delete //.
+Qed.
+
+Lemma sem_row_to_prot_bot {Σ} :
+  ⊢ iEff_le (⟦ ⟨⟩ ⟧)%R (⊥ : iEff Σ).
+Proof.
+  rewrite /sem_row_to_prot. iIntros (??) "!#".
+  simpl. iIntros "(% & % & % & % & _ & H & _)".
+  rewrite lookup_empty. 
+  iDestruct "H" as "%". inversion H.
+Qed.
+
+Lemma row_le_refl {Σ} (ρ : sem_row Σ) :
+  ⊢ ρ ≤R ρ.
+Proof.
+  iIntros (l s σ) "H".
+  iExists σ. iFrame. iApply sig_le_refl.
+Qed.
+
+Lemma row_le_trans {Σ} (ρ₁ ρ₂ ρ₃ : sem_row Σ) :
+  ρ₁ ≤R ρ₂ -∗ 
+  ρ₂ ≤R ρ₃ -∗
+  ρ₁ ≤R ρ₃.
+Proof.
+  iIntros "Hρ₁₂ Hρ₂₃".
+  iIntros (l s σ₁) "Hlookup".
+  iDestruct ("Hρ₁₂" with "Hlookup") as "(%σ₂ & Hlookup & Hσ₁₂)".
+  iDestruct ("Hρ₂₃" with "Hlookup") as "(%σ₃ & Hlookup & Hσ₂₃)".
+  iExists σ₃. iFrame. iApply (sig_le_trans with "Hσ₁₂ Hσ₂₃").
+Qed.
+
+Lemma row_le_nil {Σ} (ρ : sem_row Σ) : 
+  ⊢ ⟨⟩ ≤R ρ.
+Proof.
+  iIntros (l s σ) "Hlookup". rewrite lookup_empty. 
+  iDestruct "Hlookup" as %H. inv H.
+Qed.
+
+Lemma row_le_interp {Σ} (ρ ρ' : sem_row Σ) :
+  ρ ≤R ρ' -∗ iEff_le ⟦ ρ ⟧%R ⟦ ρ' ⟧%R.
+Proof.
+  rewrite /sem_row_to_prot /=.
+  iIntros "#Hle !# %v %Φ (%w & %l & %s & %σ & #Heq & #Hlookup & Hσ)".
+  iDestruct ("Hle" $! l s σ with "Hlookup") as "(%σ' & #Hlookup' & [_ Hσle])".
+  iExists w, l, s, σ'. iFrame "∗#". by iApply "Hσle".
+Qed.
+
+Lemma row_le_interp_to_os {Σ} (ρ ρ' : sem_row Σ) :
+  ρ ≤R ρ' -∗ iEff_le ⟦ filter_row_to_os ρ ⟧%R ⟦ filter_row_to_os ρ' ⟧%R.
+Proof.
+  rewrite /sem_row_to_prot /=.
+  iIntros "#Hle !# %v %Φ (%w & %l & %s & %σ & #Heq & #Hlookup & Hσ)".
+  iDestruct (filter_row_to_os_lookup ρ l s σ) as "[Hto _]".
+  iDestruct ("Hto" with "Hlookup") as "[Hlookup' HσOS]".
+  iDestruct ("Hle" $! l s σ with "Hlookup'") as "(%σ' & #Hlookup'' & [Hmle Hσle])".
+  iExists w, l, s, σ'. iFrame "∗#". iSplitR; last by iApply "Hσle".
+  iApply filter_row_to_os_lookup. iFrame "#".
+  iRewrite "HσOS" in "Hmle". iDestruct "Hmle" as "[H|H]".
+  { by iRewrite "H". }
+  iDestruct "H" as "%". discriminate.
+Qed.
+
+Lemma sem_row_mode_os {Σ} (ρ : gmap (string * nat) (sem_sig Σ)) :
+  (MODE ρ ≡ OS : iProp Σ) ∗-∗ ∀ l s σ, (ρ !! (l, s)) ≡ Some σ -∗ σ.1 ≡ OS.
+Proof. 
+  iInduction ρ as [|[l s] σ] "IH" using map_ind; iSplit. 
+  - iIntros "%Hmd". iIntros (???) "H".
+    rewrite lookup_empty. iDestruct "H" as %H. inv H.
+  - done.
+  - iDestruct "IH" as "[IH1 IH2]".
+    iIntros "%Hmd".
+    assert (Heq : m = delete (l, s) m).
+    { by rewrite delete_notin; last done. }
+    rewrite Heq row_mode_ins_delete /= -Heq in Hmd.
+    destruct σ.1 eqn:Hσ; last inv Hmd; simpl in Hmd.
+    iIntros (l' s' σ') "#Hlookup". 
+    destruct (decide ((l, s) = (l', s'))).
+    + rewrite - !e. rewrite lookup_insert.
+      iDestruct (option_equivI with "Hlookup") as "#Hlookup'".
+      iRewrite - "Hlookup'". by rewrite Hmd.
+    + rewrite lookup_insert_ne; last done.
+      iApply "IH1"; first by rewrite Hmd.
+      iApply "Hlookup".
+  - iDestruct "IH" as "[IH1 IH2]".
+    iIntros "H". 
+    assert (Heq : m = delete (l, s) m).
+    { by rewrite delete_notin; last done. }
+    rewrite Heq row_mode_ins_delete /= -Heq.
+    destruct σ.1 eqn:Hσ; simpl.
+    + iApply "IH2". iIntros (l' s' σ') "Hlookup".
+      destruct (decide ((l, s) = (l', s'))).
+      { rewrite - e. rewrite H. iDestruct "Hlookup" as "%H'". inv H'. }
+      iApply "H". by rewrite lookup_insert_ne; last done.
+    + iDestruct ("H" $! l s σ with "[]") as "%"; first rewrite lookup_insert //. 
+      by rewrite Hσ in H0.
+Qed.
+
+Lemma sem_row_mode_ms {Σ} (ρ : gmap (string * nat) (sem_sig Σ)) :
+  (MODE ρ ≡ MS : iProp Σ) ∗-∗ ∃ l s σ, (ρ !! (l, s)) ≡ Some σ ∗ σ.1 ≡ MS.
+Proof. 
+  iInduction ρ as [|[l s] σ] "IH" using map_ind; iSplit. 
+  - iIntros "%Hmd"; discriminate. 
+  - iIntros "(% & % & % & H & _)".
+    rewrite lookup_empty. iDestruct "H" as %H. inv H.
+  - iDestruct "IH" as "[IH1 IH2]".
+    iIntros "%Hmd".
+    assert (Heq : m = delete (l, s) m).
+    { by rewrite delete_notin; last done. }
+    destruct σ.1 eqn:Hσ'.
+    2: { iExists l, s, σ. iSplit; first by rewrite lookup_insert. by rewrite Hσ'. }
+    rewrite Heq row_mode_ins_delete Hσ' /= -Heq in Hmd.
+    iDestruct ("IH1" with "[]") as "(%l' & %s' & %σ' & Hlookup & Hσ')".
+    { by rewrite Hmd. }
+    iExists l', s', σ'. iFrame "#".
+    destruct (decide ((l, s) = (l', s'))).
+    { rewrite - !e. rewrite H. iDestruct "Hlookup" as %?. inv H0. }
+    by rewrite lookup_insert_ne; last done. 
+  - iDestruct "IH" as "[IH1 IH2]".
+    iIntros "(%l' & %s' & %σ' & Hlookup & HσOS)". 
+    assert (Heq : m = delete (l, s) m).
+    { by rewrite delete_notin; last done. }
+    rewrite Heq row_mode_ins_delete /= -Heq.
+    destruct σ.1 eqn:Hσ; simpl; last done.
+    iApply "IH2". 
+    destruct (decide ((l, s) = (l', s'))).
+    { rewrite - !e. rewrite lookup_insert. 
+      iDestruct (option_equivI with "Hlookup") as "#Hlookup'".
+      iRewrite - "Hlookup'" in "HσOS".
+      iDestruct "HσOS" as "%". rewrite Hσ in H0. discriminate. }
+    rewrite lookup_insert_ne; last done.
+    iExists l', s', σ'. iFrame.
+Qed.
+
+Lemma row_tun_ins {Σ} l s σ (ρ : sem_row Σ) :
+  (⦗ insert (l, s) σ ρ ⦘ = insert (l, S s) σ ⦗ ρ ⦘)%R. 
+Proof.
+  rewrite {1} /sem_row_tun /=. rewrite (kmap_insert _ ρ (l, s) σ) //.
+Qed.
+
+Lemma row_os_ins_gen {Σ} l s σ (ρ : sem_row Σ) :
+  (¡ (insert (l, s) σ ρ))%R = insert (l, s) (¡ σ)%S (¡ ρ)%R.
+Proof. rewrite /sem_row_os fmap_insert //. Qed.
+
+Corollary row_os_ins {Σ} l σ (ρ : sem_row Σ) :
+  (¡ ((l, σ) · ρ))%R = ((l, ¡ σ)%S · (¡ ρ))%R.
+Proof. apply row_os_ins_gen. Qed.
+
+Lemma mode_tun {Σ} (ρ : sem_row Σ) :
+  MODE ⦗ ρ ⦘ = MODE ρ.
+Proof. 
+  apply (map_ind (λ ρ, MODE ⦗ ρ ⦘ = MODE ρ)); first done.
+  intros [l s] σ ρ' Hlookup IH.
+  - rewrite row_tun_ins. 
+    rewrite - insert_delete_insert - (insert_delete_insert _ (l, S s)). 
+    rewrite !row_mode_ins_delete !delete_notin; [by rewrite IH|done|].
+    rewrite /sem_row_tun.  
+    replace (l, S s) with (sem_row_tun_f (l, s)); last done.
+    rewrite lookup_kmap //.
+Qed.
+
+Lemma mode_tun_os_comm {Σ} (ρ : sem_row Σ) :
+  (¡ ⦗ ρ ⦘)%R = (⦗ ¡ ρ ⦘)%R.
+Proof. 
+  apply (map_ind (λ ρ, ¡ ⦗ ρ ⦘ = ⦗ ¡ ρ ⦘)%R).
+  { rewrite /sem_row_tun /sem_row_os kmap_empty fmap_empty //. }
+  intros [l s] σ ρ' Hlookup IH.
+  rewrite row_tun_ins.
+  rewrite !row_os_ins_gen IH row_tun_ins //.
+Qed.
+
+Lemma row_le_ins {Σ} (ρ ρ' : sem_row Σ) (l : string) (σ σ' : sem_sig Σ) : 
+  ρ ≤R ρ' -∗ σ ≤S σ' -∗
+  (l, σ) · ρ ≤R (l, σ') · ρ'.
+Proof.
+  iIntros "#Hρρ' #Hσσ'".
+  iIntros (l'' s'' σ'') "#Hlookup".
+  destruct (decide (l = l'')) as [->|].
+  - rewrite /sem_row_ins /=. destruct s''.
+    + rewrite lookup_insert. 
+      iExists σ'. rewrite lookup_insert.
+      iSplitR; first done.
+      iDestruct (option_equivI with "Hlookup") as "#Hlookup'".
+      by iRewrite - "Hlookup'".
+    + rewrite lookup_insert_ne; last done.
+      iSpecialize ("Hρρ'" $! l'' (S s'') σ'' with "Hlookup").
+      rewrite lookup_insert_ne; last done.
+      iFrame "#".
+  - rewrite lookup_insert_ne; last (intros H; inv H).
+    iSpecialize ("Hρρ'" $! l'' s'' σ'' with "Hlookup").
+    rewrite lookup_insert_ne; last (intros H; inv H).
+    iFrame "#".
+Qed.
+
+Lemma row_le_del {Σ} (ρ : sem_row Σ) (l : string) (σ : sem_sig Σ) : 
+  ρ !! (l, 0) ≡ None -∗
+  ρ ≤R (l, σ) · ρ. 
+Proof. 
+  iIntros "#Hlookup".
+  iIntros (l' s' σ') "#Hlookup'". 
+  destruct (decide ((l, 0) = (l', s'))).
+  - rewrite <- e. 
+    iAssert (Some σ' ≡ None)%I as "Hlookup''".
+    { by iRewrite - "Hlookup'". }
+    iDestruct (option_equivI with "Hlookup''") as "[]". 
+  - iExists σ'. rewrite lookup_insert_ne; last done.
+    iFrame "#". iApply sig_le_refl.
+Qed.
+
+Lemma row_le_del_tun {Σ} (ρ : sem_row Σ) (l : string) (σ : sem_sig Σ) : 
+  ⊢ ⦗ ρ ⦘ ≤R (l, σ) · ⦗ ρ ⦘. 
+Proof. 
+  iApply row_le_del. rewrite /sem_row_tun.
+  pose proof (lookup_kmap_None sem_row_tun_f ρ (l, 0)) as [_ H].
+  rewrite H; first done.
+  intros i Hlookup. inv Hlookup.
+Qed.
+
+Lemma row_le_tun {Σ} (ρ ρ' : sem_row Σ) :
+  ρ ≤R ρ' -∗
+  ⦗ ρ ⦘ ≤R ⦗ ρ' ⦘. 
+Proof. 
+  iIntros "Hle %l %s %σ Hlookup".
+  destruct s.
+  - destruct (lookup_kmap_None sem_row_tun_f ρ (l, 0)) as [_ H].
+    rewrite H; first (iDestruct "Hlookup" as "%H'"; inv H').
+    intros [l' s'] H'. inv H'. 
+  - rewrite /sem_row_tun.
+    assert (Heq : (l, S s) = (sem_row_tun_f (l, s))) by done.
+    rewrite Heq !lookup_kmap.
+    by iApply "Hle".
+Qed.
+
+Lemma row_le_os_comp {Σ} (ρ ρ' : sem_row Σ) :
+  ρ ≤R ρ' -∗
+  ¡ ρ ≤R ¡ ρ'. 
+Proof. Admitted.
+
+Lemma row_le_os {Σ} (ρ : sem_row Σ) `{OSRow ρ} :
+  ⊢ ρ ≤R ¡ ρ. 
+Proof. Admitted.
+
+Lemma row_le_os_inv {Σ} (ρ : sem_row Σ) :
+  ⊢ ¡ ρ ≤R ρ. 
+Proof. Admitted.
+
+Lemma row_le_swap_second {Σ} (l l' : string) (σ σ' : sem_sig Σ) (ρ : sem_row Σ) : 
+  l ≠ l' →
+  ⊢ (l, σ) · (l', σ') · ρ ≤R (l', σ') · (l, σ) · ρ. 
+Proof. 
+  iIntros (Heq). rewrite /sem_row_ins /= insert_commute;
+  first iApply row_le_refl. 
+  intros ?. inv H.
+Qed.
+
+Lemma row_le_swap_third {Σ} (l l' l'' : string) (σ σ' σ'' : sem_sig Σ) (ρ : sem_row Σ) : 
+  l ≠ l' → l' ≠ l'' → l'' ≠ l →
+  ⊢ (l, σ) · (l', σ') · (l'', σ'') · ρ ≤R 
+    (l'', σ'') · (l, σ) · (l', σ') · ρ. 
+Proof. 
+  iIntros (???). rewrite /sem_row_ins /= (insert_commute _ (l',0) (l'',0)); last (intros H'; inv H').
+  rewrite (insert_commute _ (l, 0) (l'', 0)); last (intros H''; inv H'').
+  iApply row_le_refl. 
+Qed.
+
+Lemma row_le_swap_fourth {Σ} (l l' l'' l''' : string) (σ σ' σ'' σ''': sem_sig Σ) (ρ : sem_row Σ) : 
+  l ≠ l' → l ≠ l'' → l ≠ l''' → l' ≠ l'' → l' ≠ l''' → l'' ≠ l''' → 
+  ⊢ (l, σ) · (l', σ') · (l'', σ'') · (l''', σ''') · ρ ≤R 
+    (l''', σ''') · (l, σ) · (l', σ') · (l'', σ'') · ρ.
+Proof. 
+  iIntros (??????). 
+  rewrite /sem_row_ins /= (insert_commute _ (l'',0) (l''',0)); last (intros H'; inv H').
+  rewrite (insert_commute _ (l', 0) (l''', 0)); last (intros H'; inv H').
+  rewrite (insert_commute _ (l, 0) (l''', 0)); last (intros H'; inv H').
+  iApply row_le_refl. 
+Qed.
