theories/logic/sem_types.v
@@ -1,7 +1,7 @@
 
 (* sem_types.v *)
 
-(* This file contains the definition of semantic types and signatures,
+(* This file contains the definition of semantic types,
    together with the definition of base types and type formers.  
 *)
 
@@ -16,7 +16,7 @@ From hazel.program_logic Require Import weakest_precondition
 
 (* Local imports *)
 From haffel.lib Require Import logic.
-From haffel.lang Require Import hazel.
+From haffel.lang Require Import haffel.
 From haffel.lang Require Import subst_map.
 From haffel.logic Require Import iEff.
 From haffel.logic Require Import sem_def.
